src/example/treiber/ClientSpecHOCAP.v
@@ -5,7 +5,7 @@ From Fairness Require Import pind Axioms ITreeLib Red TRed IRed2 WFLibLarge.
 From Fairness Require Import FairBeh Mod Concurrency Linking.
 From Fairness Require Import PCM IProp IPM IPropAux.
 From Fairness Require Import IndexedInvariants OpticsInterp SimWeakest SimWeakestAdequacy.
-From Fairness Require Import TemporalLogic SCMemSpec ghost_map ghost_excl LifetimeRA AuthExclsRA.
+From Fairness Require Import TemporalLogic SCMemSpec ghost_map ghost_var ghost_excl LifetimeRA AuthExclsRA.
 From Fairness.treiber Require Import ClientCode SpecHOCAP.
 
 Section SPEC.
@@ -23,13 +23,17 @@ Section SPEC.
   Context {HasMemRA: @GRA.inG memRA Γ}.
   Context {HasLifetime : @GRA.inG Lifetime.t Γ}.
 
-  Context {HasAuthExclsRAlist : @GRA.inG (AuthExcls.t (list SCMem.val)) Γ}.
+  Context {HasAuthExcls : @GRA.inG (AuthExcls.t (nat * nat)) Γ}.
+
+  Context {HasGhostVar : @GRA.inG (ghost_varURA (list SCMem.val)) Γ}.
   Context {HasGhostMap : @GRA.inG (ghost_mapURA nat maybe_null_ptr) Γ}.
   Context {HasGhostExcl : @GRA.inG (ghost_exclURA unit) Γ}.
 
-  Ltac red_tl_all := red_tl; red_tl_memra; red_tl_authexcls; red_tl_lifetime; red_tl_ghost_excl_ura.
+  Ltac red_tl_all := red_tl; red_tl_memra; red_tl_lifetime; red_tl_ghost_excl_ura.
 
   Import TreiberClient.
+
+  Local Opaque s.
 
   (** Invariants. *)
 
@@ -39,28 +43,24 @@ Section SPEC.
   Definition nTMod : namespace := (nroot .@"TMod").
 
   Definition push_then_pop n γs γpop : sProp n :=
-    (○ γs [(1 : SCMem.val)] ∨ GEx γpop tt)%S.
+    (TStack n γs [(1 : SCMem.val)] ∨ GEx γpop tt)%S.
 
   Definition push_then_pop_inv n γs γpop : sProp n :=
     (syn_inv n nTpush (push_then_pop n γs γpop))%S.
 
-  Definition ClientStackState n γk k γs γpop : sProp n :=
-    (◆[k,2] ∗
-    ((live γk k (1/2) ∗ ○ γs ([] : list SCMem.val)) -U-[k](0)-◇ (dead γk k ∗ push_then_pop_inv n γs γpop))
+  Definition CState n γk k γs γpop : sProp n :=
+    (((live γk k (1/2) ∗ TStack n γs ([] : list SCMem.val)) -U-[k](0)-◇ (dead γk k ∗ push_then_pop_inv n γs γpop))
     )%S.
 
   Definition CInv n γk k γs γpop : sProp n :=
-    (syn_inv n nTCli (ClientStackState n γk k γs γpop))%S.
+    (◆[k,3,6]∗ syn_inv n nTCli (CState n γk k γs γpop))%S.
 
   Global Instance CInv_persistent n γk k γs γpop : Persistent ⟦CInv n γk k γs γpop, n⟧.
-  Proof.
-    unfold Persistent. iIntros "H". unfold CInv. rewrite red_syn_inv.
-    iDestruct "H" as "#H". auto.
-  Qed.
+  Proof. unfold Persistent,CInv. red_tl. rewrite red_syn_inv. iIntros "#$". Qed.
 
   (** Simulation proof. *)
 
-  Lemma TreiberClient_push_spec tid n :
+  Lemma TreiberClient_push_sim tid n :
     ⊢ ⟦(∀ (γk kt k γs γpop : τ{nat, 1+n}),
       ((syn_tgt_interp_as n sndl (fun m => s_memory_black m)) ∗
       (⤉ IsT nTMod n 1 2 s kt γs) ∗
@@ -79,13 +79,14 @@ Section SPEC.
     )%S,1+n⟧.
   Proof.
     iIntros.
-    red_tl_all; iIntros (γk); red_tl_all; iIntros (kt); red_tl_all; iIntros (k); red_tl_all; iIntros (γs); red_tl_all; iIntros (γpop).
+    red_tl; iIntros (γk); red_tl; iIntros (kt); red_tl; iIntros (k);
+    red_tl; iIntros (γs); red_tl; iIntros (γpop).
 
-    red_tl_all. unfold CInv. simpl.
+    unfold CInv. red_tl_all. simpl.
 
     iEval (rewrite red_syn_inv; rewrite red_syn_wpsim; rewrite red_syn_tgt_interp_as).
 
-    iIntros "(#Mem & #IsTreiber & #CInv & TID & Pck & Duty & Pc & Live & k_Act)".
+    iIntros "(#Mem & #IsTreiber & #[Ob_kb CInv] & TID & Pck & Duty & Pc & Live & k_Act)".
 
     unfold fn2th. simpl. unfold thread_push, TreiberClientSpec.thread_push.
     rred2r. lred2r.
@@ -106,23 +107,22 @@ Section SPEC.
       iIntros (s_st). red_tl_all. iIntros "[TStackInv _]".
       rewrite red_syn_fupd. red_tl_all.
       iInv "CInv" as "Client" "CloseCInv".
-      iEval (unfold ClientStackState; simpl; red_tl_all; simpl; rewrite red_syn_until_tpromise) in "Client".
+      iEval (unfold CState; simpl; red_tl_all; simpl; rewrite red_syn_until_tpromise) in "Client".
       iDestruct "Client" as "[#OBL PushProm]".
 
       iEval (unfold until_thread_promise; red_tl_all; simpl) in "PushProm".
 
-      iDestruct "PushProm" as "[#Prm [Bf | #Af]]"; simpl.
+      iDestruct "PushProm" as "[Bf | #Af]"; simpl.
       - iEval (red_tl_all; simpl) in "Bf". iDestruct "Bf" as "[LiveInv TStackC]".
-        iDestruct (AuthExcls.b_w_eq with "TStackInv TStackC") as "%EQ".
-        subst s_st.
-        iMod (AuthExcls.b_w_update with "TStackInv TStackC") as "[TStackInv TStackC]".
+        iDestruct (TStack_agree with "TStackInv TStackC") as %->.
+        iMod (TStack_update with "TStackInv TStackC") as "[TStackInv TStackC]".
         iMod ((FUpd_alloc _ _ _ n (nTpush) (push_then_pop n γs γpop : sProp n)%S) with "[TStackC]") as "#Pushed"; [lia| |].
         { unfold push_then_pop. iEval (simpl; red_tl_all; simpl). auto. }
         iDestruct (Lifetime.pending_merge with "Live LiveInv") as "Live".
         iEval (rewrite Qp.half_half) in "Live".
         iMod (Lifetime.pending_shot with "Live") as "#Dead".
         iMod ("CloseCInv" with "[]") as "_".
-        { iEval (unfold ClientStackState; simpl; red_tl_all; simpl).
+        { iEval (unfold CState; simpl; red_tl_all; simpl).
           iFrame "#". iEval (rewrite red_syn_until_tpromise).
           iApply until_tpromise_make2. simpl. iSplit; auto.
           iEval (red_tl_all; simpl). iModIntro; iSplit; auto.
@@ -148,7 +148,7 @@ Section SPEC.
     iEval (unfold term_cond). iSplit; iFrame. iPureIntro; auto.
   Qed.
 
-  Lemma TreiberClient_pop_spec tid n :
+  Lemma TreiberClient_pop_sim tid n :
     ⊢ ⟦(∀ (γk k kt γs γpop : τ{nat, 1+n}),
       ((syn_tgt_interp_as n sndl (fun m => s_memory_black m)) ∗
       (⤉ IsT nTMod n 1 2 s kt γs) ∗
@@ -166,15 +166,16 @@ Section SPEC.
     )%S,1+n⟧.
   Proof.
     iIntros.
-    red_tl_all; iIntros (γk); red_tl_all; iIntros (k);
-    red_tl_all; iIntros (kt);
-    red_tl_all; iIntros (γs); red_tl_all; iIntros (γpop).
+    red_tl; iIntros (γk); red_tl; iIntros (k); red_tl; iIntros (kt);
+    red_tl; iIntros (γs); red_tl; iIntros (γpop).
 
-    red_tl_all. unfold CInv. simpl.
+    unfold CInv. red_tl_all. simpl.
 
     iEval (rewrite red_syn_inv; rewrite red_syn_wpsim; rewrite red_syn_tgt_interp_as).
 
-    iIntros "(#Mem & #IsTreiber & #CInv & Tok & Pck & TID & Duty)".
+    iIntros "(#Mem & #IsTreiber & #[Ob_kb CInv] & Tok & Pck & TID & Duty)".
+
+    iMod (ccs_make_fine _ _ _ [] 0 with "[$Ob_kb]") as "CCS".
 
     unfold fn2th. simpl. unfold thread_pop, TreiberClientSpec.thread_pop.
     rred2r. lred2r.
@@ -185,19 +186,16 @@ Section SPEC.
     iApply (wpsim_yieldR with "[$Duty]"); [lia|].
     iIntros "Duty _". rred2r. iApply wpsim_tauR. rred2r.
 
-    iInv "CInv" as "Client" "CloseCInv".
-    iEval (unfold ClientStackState; simpl; red_tl_all; simpl; rewrite red_syn_until_tpromise) in "Client".
+    iInv "CInv" as "PushProm" "CloseCInv".
+    iEval (unfold CState; simpl; red_tl_all; simpl; rewrite red_syn_until_tpromise) in "PushProm".
 
-    iDestruct "Client" as "[#Obl PushProm]".
-    iPoseProof (until_tpromise_get_tpromise with "PushProm") as "#TProm".
+    iDestruct (until_tpromise_get_tpromise with "PushProm") as "#TProm".
     iRevert "Tok TID Duty CloseCInv Pck".
-    iMod (until_tpromise_ind with "[Obl PushProm] [-]") as "Ind"; cycle 2.
-    { iApply "Ind". }
-    { iSplit; iFrame; auto. }
+    iMod (ccs_until_tpromise_ind with "[$CCS $PushProm] [-]") as "Ind"; [|by iApply "Ind"].
     iSplit.
-    - simpl. red_tl_all. iIntros "!> IH !> [LiveInv TStackC] Tok TID Duty CloseCInv Pck".
+    - simpl. red_tl_all. iIntros "!> IH !> _ [LiveInv TStackC] Tok TID Duty CloseCInv Pck".
       iMod ("CloseCInv" with "[LiveInv TStackC]") as "_".
-      { iEval (unfold ClientStackState; simpl; red_tl_all; simpl).
+      { iEval (unfold CState; simpl; red_tl_all; simpl).
         iFrame "#". iEval (rewrite red_syn_until_tpromise).
         unfold until_thread_promise. simpl. iSplit; auto.
         iLeft. red_tl_all. iFrame.
@@ -209,17 +207,17 @@ Section SPEC.
         iIntros (s_st). red_tl_all. iIntros "[TStackInv _]".
         rewrite red_syn_fupd. red_tl_all.
         iInv "CInv" as "Client" "CloseCInv".
-        iEval (unfold ClientStackState; simpl; red_tl_all; simpl; rewrite red_syn_until_tpromise) in "Client".
+        iEval (unfold CState; simpl; red_tl_all; simpl; rewrite red_syn_until_tpromise) in "Client".
 
         iDestruct "Client" as "[#OBL PushProm]".
 
         iEval (unfold until_thread_promise; red_tl_all; simpl) in "PushProm".
-        iDestruct "PushProm" as "[#Prm [Bf | #Af]]"; simpl.
+        iDestruct "PushProm" as "[Bf | #Af]"; simpl.
         - iEval (red_tl_all; simpl) in "Bf". iDestruct "Bf" as "[LiveInv TStackC]".
-          iDestruct (AuthExcls.b_w_eq with "TStackInv TStackC") as "%EQ".
+          iDestruct (TStack_agree with "TStackInv TStackC") as "%EQ".
           subst s_st.
           iMod ("CloseCInv" with "[LiveInv TStackC]") as "_".
-          { iEval (unfold ClientStackState; simpl; red_tl_all; simpl).
+          { iEval (unfold CState; simpl; red_tl_all; simpl).
             iFrame "#". iEval (rewrite red_syn_until_tpromise).
             unfold until_thread_promise. simpl. iSplit; auto.
             iLeft. red_tl_all. iFrame.
@@ -231,12 +229,12 @@ Section SPEC.
           unfold push_then_pop. simpl. red_tl_all.
           iDestruct "TStackC" as "[TStackC| Tokt]"; last first.
           { by iDestruct (ghost_excl_exclusive with "Tok Tokt") as "%False". }
-          iDestruct (AuthExcls.b_w_eq with "TStackInv TStackC") as "%EQ".
+          iDestruct (TStack_agree with "TStackInv TStackC") as "%EQ".
           subst s_st.
-          iMod (AuthExcls.b_w_update with "TStackInv TStackC") as "[TStackInv TStackC]".
+          iMod (TStack_update with "TStackInv TStackC") as "[TStackInv TStackC]".
           iMod ("ClosePushedInv" with "[$Tok]") as "_".
           iMod ("CloseCInv" with "[TStackC]") as "_".
-          { iEval (unfold ClientStackState; simpl; red_tl_all; simpl).
+          { iEval (unfold CState; simpl; red_tl_all; simpl).
             iFrame "#". iEval (rewrite red_syn_until_tpromise).
             unfold until_thread_promise. simpl. iSplit; auto.
             iRight. red_tl_all. iFrame "#".
@@ -256,16 +254,15 @@ Section SPEC.
         iEval (rewrite unfold_iter_eq; rred2r).
         iApply (wpsim_yieldR with "[$Duty]"); [lia|].
         iIntros "Duty C". lred2r. rred2r. iApply wpsim_tauR. rred2r.
-        iInv "CInv" as "Client" "CloseCInv".
-        iEval (unfold ClientStackState; simpl; red_tl_all; simpl; rewrite red_syn_until_tpromise) in "Client".
+        iInv "CInv" as "PushProm" "CloseCInv".
+        iEval (unfold CState; simpl; red_tl_all; simpl; rewrite red_syn_until_tpromise) in "PushProm".
 
-        iDestruct "Client" as "[_ PushProm]".
         iMod ("IH" with "[$C $PushProm] ") as "IH".
         iApply ("IH" with "Tok TID Duty CloseCInv Pck").
     - unfold push_then_pop_inv. simpl. red_tl_all. rewrite red_syn_inv.
       iIntros "!> #[Dead PushedInv] Tok TID Duty CloseCInv Pck".
       iMod ("CloseCInv" with "[]") as "_".
-      { iEval (unfold ClientStackState; simpl; red_tl_all; simpl).
+      { iEval (unfold CState; simpl; red_tl_all; simpl).
         iFrame "#". iEval (rewrite red_syn_until_tpromise).
         iApply until_tpromise_make2. simpl. iSplit; auto.
         iEval (red_tl_all; simpl). iModIntro; iSplit; auto.
@@ -275,12 +272,12 @@ Section SPEC.
       iFrame. iSplitL; [|done]. iIntros (s_st). red_tl_all. iIntros "[TStackInv _]".
       rewrite red_syn_fupd. red_tl_all.
       iInv "CInv" as "Client" "CloseCInv".
-      iEval (unfold ClientStackState; simpl; red_tl_all; simpl; rewrite red_syn_until_tpromise) in "Client".
+      iEval (unfold CState; simpl; red_tl_all; simpl; rewrite red_syn_until_tpromise) in "Client".
 
       iDestruct "Client" as "[#OBL PushProm]".
 
       iEval (unfold until_thread_promise; red_tl_all; simpl) in "PushProm".
-      iDestruct "PushProm" as "[#Prm [Bf | _]]"; simpl.
+      iDestruct "PushProm" as "[Bf | _]"; simpl.
       - iEval (red_tl_all; simpl) in "Bf". iDestruct "Bf" as "[LiveInv TStackC]".
         iDestruct (Lifetime.pending_not_shot with "LiveInv Dead") as "%False".
         done.
@@ -289,11 +286,11 @@ Section SPEC.
         unfold push_then_pop. simpl. red_tl_all.
         iDestruct "TStackC" as "[TStackC| Tokt]"; last first.
         { iDestruct (ghost_excl_exclusive with "Tok Tokt") as %[]. }
-        iDestruct (AuthExcls.b_w_eq with "TStackInv TStackC") as %->.
-        iMod (AuthExcls.b_w_update with "TStackInv TStackC") as "[TStackInv TStackC]".
+        iDestruct (TStack_agree with "TStackInv TStackC") as %->.
+        iMod (TStack_update with "TStackInv TStackC") as "[TStackInv TStackC]".
         iMod ("ClosePushedInv" with "[$Tok]") as "_".
-        iMod ("CloseCInv" with "[TStackC]") as "_".
-        { iEval (unfold ClientStackState; simpl; red_tl_all; simpl).
+        iMod ("CloseCInv" with "[]") as "_".
+        { iEval (unfold CState; simpl; red_tl_all; simpl).
           iFrame "#". iEval (rewrite red_syn_until_tpromise).
           unfold until_thread_promise. simpl. iSplit; auto.
           iRight. red_tl_all. iFrame "#".
@@ -309,5 +306,130 @@ Section SPEC.
     iEval (unfold term_cond). iSplit; iFrame. iPureIntro; auto.
     Unshelve. all: apply ndot_ne_disjoint; ss.
   Qed.
+
+(* Note: Proof is same for HOCAP and LAT *)
+Section INITIAL.
+
+  Variable tid_push tid_pop : thread_id.
+  Let init_ord := Ord.O.
+  Let init_ths :=
+        (NatStructsLarge.NatMap.add
+            tid_push tt
+            (NatStructsLarge.NatMap.add
+              tid_pop tt
+              (NatStructsLarge.NatMap.empty unit))).
+
+  Let idx := 1.
+
+  Lemma init_sat E (H_TID : tid_push ≠ tid_pop) :
+    (OwnM (memory_init_resource TreiberClient.gvs))
+      ∗ (OwnM (AuthExcls.rest_ra (gt_dec 0) (0, 0)))
+      ∗
+      (WSim.initial_prop
+        TreiberClientSpec.module TreiberClient.module
+          (Vars:=@sProp STT Γ) (Σ:=Σ)
+          (STATESRC:=@SRA.in_subG Γ Σ sub _ _STATESRC)
+          (STATETGT:=@SRA.in_subG Γ Σ sub _ _STATETGT)
+          (IDENTSRC:=@SRA.in_subG Γ Σ sub _ _IDENTSRC)
+          (IDENTTGT:=@SRA.in_subG Γ Σ sub _ _IDENTTGT)
+          (ARROWRA:=@_ARROWRA STT Γ Σ TLRAS)
+          idx init_ths init_ord)
+      ⊢
+      =| 1+idx |=(⟦syn_fairI (1+idx), 1+idx⟧)={E}=>
+        ∃ (γk k γpop γs kt : nat),
+        ⟦syn_tgt_interp_as idx sndl (fun m => s_memory_black m),1+idx⟧ ∗
+        ⟦IsT nTMod idx 1 2 s kt γs,idx⟧ ∗
+        ⟦CInv idx γk k γs γpop,idx ⟧ ∗
+        (* thread_push *)
+        own_thread tid_push ∗
+        ⟦Duty(tid_push) [(k, 0, (dead γk k : sProp idx) ∗ push_then_pop_inv idx γs γpop)],idx⟧ ∗
+        ◇[kt](1, 1) ∗
+        ◇[k](3, 5) ∗
+        live γk (k : nat) (1/2) ∗
+        ⋈[k] ∗
+        (* thread_pop *)
+        GEx γpop tt ∗
+        ◇[kt](1,1) ∗
+        own_thread tid_pop ∗
+        ⟦Duty(tid_pop) [],idx⟧
+  .
+  Proof.
+    iIntros "(Mem & _ & Init)". rewrite red_syn_fairI.
+    iDestruct (memory_init_iprop with "Mem") as "[Mem ↦s]".
+    iDestruct "↦s" as "((s↦ & _) & _)".
+    Local Transparent s.
+    iEval (simpl; fold s) in "s↦".
+    Local Opaque s.
+
+    unfold WSim.initial_prop.
+    iDestruct "Init" as "(_ & _ & Ds & Ts & _ & St_tgt)".
+
+    assert (NatStructsLarge.NatMap.find tid_push init_ths = Some tt) as Htid_push.
+    { unfold init_ths. apply NatStructsLarge.nm_find_add_eq. }
+    iDestruct (natmap_prop_remove_find _ _ _ Htid_push with "Ds") as "[Dpush Ds]".
+    iDestruct (natmap_prop_remove_find _ _ _ Htid_push with "Ts") as "[Tpush Ts]".
+    clear Htid_push.
+
+    assert (NatStructsLarge.NatMap.find tid_pop (NatStructsLarge.NatMap.remove tid_push init_ths) = Some tt) as Htid_pop.
+    { unfold init_ths.
+      rewrite NatStructsLarge.NatMapP.F.remove_neq_o; ss.
+      rewrite NatStructsLarge.nm_find_add_neq; ss.
+      rewrite NatStructsLarge.nm_find_add_eq. ss.
+    }
+    iDestruct (natmap_prop_remove_find _ _ _ Htid_pop with "Ds") as "[Dpop _]".
+    iDestruct (natmap_prop_remove_find _ _ _ Htid_pop with "Ts") as "[Tpop _]".
+    clear Htid_pop.
+
+    iMod (tgt_interp_as_id _ _ (n:=idx) with "[St_tgt Mem]") as "St_tgt"; [auto|..].
+    2:{ iExists _. iFrame. simpl.
+        instantiate (1:=fun '(_, m) => s_memory_black m). simpl.
+        red_tl_all. iFrame.
+    }
+    { simpl. instantiate (1:= (∃ (st : τ{st_tgt_type, idx}), ⟨Atom.ow_st_tgt st⟩ ∗ (let '(_, m) := st in s_memory_black (n:=idx) m))%S).
+      red_tl. f_equal.
+    }
+    iDestruct (tgt_interp_as_compose (n:=idx) (la:=Lens.id) (lb:=sndl) with "St_tgt") as "#TGT_ST".
+    { ss. econs. iIntros ([x m]) "MEM". unfold Lens.view. ss. iFrame.
+      iIntros (m') "MEM". iFrame.
+    }
+    iEval (rewrite Lens.left_unit) in "TGT_ST".
+    iClear "St_tgt". clear.
+
+    iMod (alloc_obligation_fine 3 6) as (k) "(#OB_kb & Pc_k & Po_k)".
+    iEval (rewrite -Qp.half_half) in "Po_k".
+    iDestruct (pending_split _ (1/2) (1/2) with "Po_k") as "(Po_d & Po_p)".
+    iDestruct (pc_split _ _ 5 1 with "Pc_k") as "[Pc_k_push Pc_k]".
+    iMod (pc_drop _ 1 3 ltac:(auto) 1 with "Pc_k") as "Pc_k"; [lia|].
+
+    iMod (Lifetime.alloc k) as (γk) "live".
+    iEval (rewrite -Qp.half_half) in "live".
+    iDestruct (Lifetime.pending_split _ (1/2) (1/2) with "live") as "[live_i live_p]".
+
+    iMod (ghost_excl_alloc tt) as (γpop) "Tok".
+    iMod (alloc_Treiber nTMod idx _ 1 2 with "s↦") as (kt γs) "(#IsT & TStack & Pc_kt)".
+    iDestruct (pc_split _ _ 1 1 with "Pc_kt") as "[? ?]".
+
+    iMod (duty_add _ _ [] _ 0 ((dead γk k : sProp idx) ∗ push_then_pop_inv idx γs γpop : sProp idx)%S with "[$Dpush $Po_d $Pc_k] []") as "Dpush".
+    { simpl. unfold push_then_pop_inv. red_tl_all.
+      rewrite red_syn_inv. iModIntro. iIntros "#$".
+    }
+
+    iDestruct (duty_delayed_tpromise with "Dpush") as "#Prm'"; [ss;eauto|].
+    iMod (activate_tpromise with "Prm' Po_p") as "[#Prm #Act_k]".
+    iClear "Prm'".
+
+    iDestruct (until_tpromise_make1 _ _ _ ((live γk k (1/2) : sProp idx) ∗ TStack idx γs [] : sProp idx)%S with "[live_i TStack]") as "uPrm".
+    { simpl. red_tl_all. iFrame "∗". iFrame "Prm". }
+
+    iMod (FUpd_alloc _ _ _ idx nTCli (CState idx γk k γs γpop) with "[uPrm]") as "#CInv"; [lia| |].
+    { simpl. unfold CState. rewrite red_syn_until_tpromise. iFrame. }
+
+    iModIntro. iExists γk,k,γpop,γs,kt.
+
+    rewrite red_syn_tgt_interp_as. iFrame "∗#".
+    unfold CInv. red_tl. rewrite red_syn_inv. iFrame "OB_kb CInv".
+  Qed.
+
+End INITIAL.
 
 End SPEC.
