src/example/treiber/ClientSpecLat.v
@@ -23,6 +23,8 @@ Section SPEC.
   Context {HasMemRA: @GRA.inG memRA Γ}.
   Context {HasLifetime : @GRA.inG Lifetime.t Γ}.
 
+  Context {HasAuthExcls : @GRA.inG (AuthExcls.t (nat * nat)) Γ}.
+
   Context {HasGhostMap : @GRA.inG (ghost_mapURA nat maybe_null_ptr) Γ}.
   Context {HasGhostVar : @GRA.inG (ghost_varURA (list SCMem.val)) Γ}.
 
@@ -31,6 +33,8 @@ Section SPEC.
   Ltac red_tl_all := red_tl; red_tl_memra; red_tl_ghost_excl_ura; red_tl_lifetime.
 
   Import TreiberClient.
+
+  Local Opaque s.
 
   (** Invariants. *)
 
@@ -45,23 +49,19 @@ Section SPEC.
   Definition push_then_pop_inv n γs γpop : sProp n :=
     (syn_inv n nTpush (push_then_pop n γs γpop))%S.
 
-  Definition Client2StackState n γk k γs γpop : sProp n :=
-    (◆[k,2] ∗
-    ((live γk k (1/2) ∗ TStack n γs ([] : list SCMem.val)) -U-[k](0)-◇ (dead γk k ∗ push_then_pop_inv n γs γpop))
+  Definition CState n γk k γs γpop : sProp n :=
+    (((live γk k (1/2) ∗ TStack n γs []) -U-[k](0)-◇ (dead γk k ∗ push_then_pop_inv n γs γpop))
     )%S.
 
   Definition CInv n γk k γs γpop : sProp n :=
-    (syn_inv n nTCli (Client2StackState n γk k γs γpop))%S.
+    (◆[k,3,6] ∗ syn_inv n nTCli (CState n γk k γs γpop))%S.
 
   Global Instance CInv_persistent n γk k γs γpop : Persistent ⟦CInv n γk k γs γpop, n⟧.
-  Proof.
-    unfold Persistent. iIntros "H". unfold CInv. rewrite red_syn_inv.
-    iDestruct "H" as "#H". auto.
-  Qed.
+  Proof. unfold Persistent,CInv. red_tl. rewrite red_syn_inv. iIntros "#$". Qed.
 
   (** Simulation proof. *)
 
-  Lemma TreiberClient_push_spec tid n :
+  Lemma TreiberClient_push_sim tid n :
     ⊢ ⟦(∀ (γk kt k γs γpop : τ{nat, 1+n}),
       ((syn_tgt_interp_as n sndl (fun m => s_memory_black m)) ∗
       (⤉ IsT nTMod n 1 2 s kt γs) ∗
@@ -80,13 +80,13 @@ Section SPEC.
     )%S,1+n⟧.
   Proof.
     iIntros.
-    red_tl_all; iIntros (γk); red_tl_all; iIntros (kt); red_tl_all; iIntros (k); red_tl_all; iIntros (γs); red_tl_all; iIntros (γpop).
+    red_tl; iIntros (γk); red_tl; iIntros (kt); red_tl; iIntros (k); red_tl; iIntros (γs); red_tl; iIntros (γpop).
 
-    red_tl_all. unfold CInv. simpl.
+    unfold CInv. red_tl_all. simpl.
 
     iEval (rewrite red_syn_inv; rewrite red_syn_wpsim; rewrite red_syn_tgt_interp_as).
 
-    iIntros "(#Mem & #IsTreiber & #CInv & TID & Pck & Duty & Pc & Live & k_Act)".
+    iIntros "(#Mem & #IsTreiber & #[Ob_kb CInv] & TID & Pck & Duty & Pc & Live & k_Act)".
 
     unfold fn2th. simpl. unfold thread_push, TreiberClientSpec.thread_push.
     rred2r. lred2r.
@@ -108,16 +108,16 @@ Section SPEC.
 
     unfold atomic_update.
 
-    iInv "CInv" as "Client2" "CloseCInv". simpl.
+    iInv "CInv" as "Client" "CloseCInv". simpl.
     iApply FUpd_mask_keep; [set_solver|].
     iIntros "CloseTS !>".
 
-    iEval (unfold Client2StackState; simpl; red_tl_all; simpl; rewrite red_syn_until_tpromise) in "Client2".
-    iDestruct "Client2" as "[#OBL PushProm]".
+    iEval (unfold CState; simpl; red_tl_all; simpl; rewrite red_syn_until_tpromise) in "Client".
+    iDestruct "Client" as "[#OBL PushProm]".
 
     iEval (unfold until_thread_promise; red_tl_all; simpl) in "PushProm".
 
-    iDestruct "PushProm" as "[#Prm [Bf | #Af]]"; simpl; last first.
+    iDestruct "PushProm" as "[Bf | #Af]"; simpl; last first.
     { iEval (red_tl_all; simpl) in "Af". iDestruct "Af" as "[Dead TStackC]".
       by iDestruct (Lifetime.pending_not_shot with "Live Dead") as "%False".
     }
@@ -130,7 +130,7 @@ Section SPEC.
     iMod (Lifetime.pending_shot with "Live") as "#Dead".
     iMod "CloseTS" as "_".
     iMod ("CloseCInv" with "[]") as "_".
-    { iEval (unfold Client2StackState; simpl; red_tl_all; simpl).
+    { iEval (unfold CState; simpl; red_tl_all; simpl).
       iFrame "#". iEval (rewrite red_syn_until_tpromise).
       iApply until_tpromise_make2. simpl. iSplit; auto.
       iEval (red_tl_all; simpl). iModIntro; iSplit; auto.
@@ -151,7 +151,7 @@ Section SPEC.
     iEval (unfold term_cond). iSplit; iFrame. iPureIntro; auto.
   Qed.
 
-  Lemma TreiberClient_pop_spec tid n :
+  Lemma TreiberClient_pop_sim tid n :
     ⊢ ⟦(∀ (γk k kt γs γpop : τ{nat, 1+n}),
       ((syn_tgt_interp_as n sndl (fun m => s_memory_black m)) ∗
       (⤉ IsT nTMod n 1 2 s kt γs) ∗
@@ -169,15 +169,16 @@ Section SPEC.
     )%S,1+n⟧.
   Proof.
     iIntros.
-    red_tl_all; iIntros (γk); red_tl_all; iIntros (k);
-    red_tl_all; iIntros (kt);
-    red_tl_all; iIntros (γs); red_tl_all; iIntros (γpop).
+    red_tl; iIntros (γk); red_tl; iIntros (k); red_tl; iIntros (kt);
+    red_tl; iIntros (γs); red_tl; iIntros (γpop).
 
-    red_tl_all. unfold CInv. simpl.
+    unfold CInv. red_tl_all. simpl.
 
     iEval (rewrite red_syn_inv; rewrite red_syn_wpsim; rewrite red_syn_tgt_interp_as).
 
-    iIntros "(#Mem & #IsTreiber & #CInv & Tok & Pck & TID & Duty)".
+    iIntros "(#Mem & #IsTreiber & #[Ob_kb CInv] & Tok & Pck & TID & Duty)".
+
+    iMod (ccs_make_fine _ _ _ [] 0 with "[$Ob_kb]") as "CCS".
 
     unfold fn2th. simpl. unfold thread_pop, TreiberClientSpec.thread_pop.
     rred2r. lred2r.
@@ -185,19 +186,16 @@ Section SPEC.
     iApply (wpsim_yieldR with "[$Duty]"); [lia|].
     iIntros "Duty _". rred2r. iApply wpsim_tauR. rred2r.
 
-    iInv "CInv" as "Client2" "CloseCInv".
-    iEval (unfold Client2StackState; simpl; red_tl_all; simpl; rewrite red_syn_until_tpromise) in "Client2".
+    iInv "CInv" as "PushProm" "CloseCInv".
+    iEval (unfold CState; simpl; red_tl_all; simpl; rewrite red_syn_until_tpromise) in "PushProm".
 
-    iDestruct "Client2" as "[#Obl PushProm]".
-    iPoseProof (until_tpromise_get_tpromise with "PushProm") as "#TProm".
+    iDestruct (until_tpromise_get_tpromise with "PushProm") as "#TProm".
     iRevert "Tok TID Duty CloseCInv Pck".
-    iMod (until_tpromise_ind with "[Obl PushProm] [-]") as "Ind"; cycle 2.
-    { iApply "Ind". }
-    { iSplit; iFrame; auto. }
+    iMod (ccs_until_tpromise_ind with "[$CCS $PushProm] [-]") as "Ind"; [|by iApply "Ind"].
     iSplit.
-    - simpl. red_tl_all. iIntros "!> IH !> [LiveInv TStackC] Tok TID Duty CloseCInv Pck".
+    - simpl. red_tl_all. iIntros "!> IH !> _ [LiveInv TStackC] Tok TID Duty CloseCInv Pck".
       iMod ("CloseCInv" with "[LiveInv TStackC]") as "_".
-      { iEval (unfold Client2StackState; simpl; red_tl_all; simpl).
+      { iEval (unfold CState; simpl; red_tl_all; simpl).
         iFrame "#". iEval (rewrite red_syn_until_tpromise).
         unfold until_thread_promise. simpl. iSplit; auto.
         iLeft. red_tl_all. iFrame.
@@ -212,13 +210,13 @@ Section SPEC.
 
       unfold atomic_update.
 
-      iInv "CInv" as "Client2" "CloseCInv". simpl.
+      iInv "CInv" as "Client" "CloseCInv". simpl.
 
-      iEval (unfold Client2StackState; simpl; red_tl_all; simpl; rewrite red_syn_until_tpromise) in "Client2".
+      iEval (unfold CState; simpl; red_tl_all; simpl; rewrite red_syn_until_tpromise) in "Client".
 
-      iDestruct "Client2" as "[#OBL PushProm]".
+      iDestruct "Client" as "[#OBL PushProm]".
       iEval (unfold until_thread_promise; red_tl_all; simpl) in "PushProm".
-      iDestruct "PushProm" as "[#Prm [Bf | #Af]]"; simpl.
+      iDestruct "PushProm" as "[Bf | #Af]"; simpl.
       + iEval (red_tl_all; simpl) in "Bf". iDestruct "Bf" as "[LiveInv TStackC]".
         iApply FUpd_mask_keep; [set_solver|].
         iIntros "CloseTS !>".
@@ -226,7 +224,7 @@ Section SPEC.
         iExists _. iFrame. iIntros (s_st) "[TStackC %EQ]". subst s_st.
         iMod "CloseTS" as "_".
         iMod ("CloseCInv" with "[LiveInv TStackC]") as "_".
-        { iEval (unfold Client2StackState; simpl; red_tl_all; simpl).
+        { iEval (unfold CState; simpl; red_tl_all; simpl).
           iFrame "#". iEval (rewrite red_syn_until_tpromise).
           unfold until_thread_promise. simpl. iSplit; auto.
           iLeft. red_tl_all. iFrame.
@@ -234,10 +232,9 @@ Section SPEC.
         iIntros "!>" (?) "[Duty Pck]".
         rred2r. iApply wpsim_tauR. rred2r.
 
-        iInv "CInv" as "Client2" "CloseCInv".
-        iEval (unfold Client2StackState; simpl; red_tl_all; simpl; rewrite red_syn_until_tpromise) in "Client2".
+        iInv "CInv" as "PushProm" "CloseCInv".
+        iEval (unfold CState; simpl; red_tl_all; simpl; rewrite red_syn_until_tpromise) in "PushProm".
 
-        iDestruct "Client2" as "[_ PushProm]".
         iMod ("IH" with "[$C $PushProm] ") as "IH".
         iApply ("IH" with "Tok TID Duty CloseCInv Pck").
       + iEval (red_tl_all; simpl) in "Af". iDestruct "Af" as "[Dead PushedInv]".
@@ -252,8 +249,8 @@ Section SPEC.
 
         iMod "CloseTS" as "_".
         iMod ("ClosePushedInv" with "[$Tok]") as "_".
-        iMod ("CloseCInv" with "[TStackC]") as "_".
-        { iEval (unfold Client2StackState; simpl; red_tl_all; simpl).
+        iMod ("CloseCInv" with "[]") as "_".
+        { iEval (unfold CState; simpl; red_tl_all; simpl).
           iFrame "#". iEval (rewrite red_syn_until_tpromise).
           unfold until_thread_promise. simpl. iSplit; auto.
           iRight. red_tl_all. iFrame "#".
@@ -267,7 +264,7 @@ Section SPEC.
   - unfold push_then_pop_inv. simpl. red_tl_all. rewrite red_syn_inv.
     iIntros "!> #[Dead PushedInv] Tok TID Duty CloseCInv Pck".
     iMod ("CloseCInv" with "[]") as "_".
-    { iEval (unfold Client2StackState; simpl; red_tl_all; simpl).
+    { iEval (unfold CState; simpl; red_tl_all; simpl).
       iFrame "#". iEval (rewrite red_syn_until_tpromise).
       iApply until_tpromise_make2. simpl. iSplit; auto.
       iEval (red_tl_all; simpl). iModIntro; iSplit; auto.
@@ -282,11 +279,11 @@ Section SPEC.
 
     unfold atomic_update.
 
-    iInv "CInv" as "Client2" "CloseCInv". simpl.
-    iEval (unfold Client2StackState; simpl; red_tl_all; simpl; rewrite red_syn_until_tpromise) in "Client2".
-    iDestruct "Client2" as "[#OBL PushProm]".
+    iInv "CInv" as "Client" "CloseCInv". simpl.
+    iEval (unfold CState; simpl; red_tl_all; simpl; rewrite red_syn_until_tpromise) in "Client".
+    iDestruct "Client" as "[#OBL PushProm]".
     iEval (unfold until_thread_promise; red_tl_all; simpl) in "PushProm".
-    iDestruct "PushProm" as "[#Prm [Bf | _]]"; simpl.
+    iDestruct "PushProm" as "[Bf | _]"; simpl.
     { iEval (red_tl_all; simpl) in "Bf". iDestruct "Bf" as "[LiveInv TStackC]".
       iDestruct (Lifetime.pending_not_shot with "LiveInv Dead") as %[].
     }
@@ -303,7 +300,7 @@ Section SPEC.
     iMod "CloseTS" as "_".
     iMod ("ClosePushedInv" with "[$Tok]") as "_".
     iMod ("CloseCInv" with "[TStackC]") as "_".
-    { iEval (unfold Client2StackState; simpl; red_tl_all; simpl).
+    { iEval (unfold CState; simpl; red_tl_all; simpl).
       iFrame "#". iEval (rewrite red_syn_until_tpromise).
       unfold until_thread_promise. simpl. iSplit; auto.
       iRight. red_tl_all. iFrame "#".
@@ -318,5 +315,130 @@ Section SPEC.
     Unshelve.
     all: apply ndot_ne_disjoint; ss.
   Qed.
+
+(* Note: Proof is same for HOCAP and LAT *)
+Section INITIAL.
+
+  Variable tid_push tid_pop : thread_id.
+  Let init_ord := Ord.O.
+  Let init_ths :=
+        (NatStructsLarge.NatMap.add
+            tid_push tt
+            (NatStructsLarge.NatMap.add
+              tid_pop tt
+              (NatStructsLarge.NatMap.empty unit))).
+
+  Let idx := 1.
+
+  Lemma init_sat E (H_TID : tid_push ≠ tid_pop) :
+    (OwnM (memory_init_resource TreiberClient.gvs))
+      ∗ (OwnM (AuthExcls.rest_ra (gt_dec 0) (0, 0)))
+      ∗
+      (WSim.initial_prop
+        TreiberClientSpec.module TreiberClient.module
+          (Vars:=@sProp STT Γ) (Σ:=Σ)
+          (STATESRC:=@SRA.in_subG Γ Σ sub _ _STATESRC)
+          (STATETGT:=@SRA.in_subG Γ Σ sub _ _STATETGT)
+          (IDENTSRC:=@SRA.in_subG Γ Σ sub _ _IDENTSRC)
+          (IDENTTGT:=@SRA.in_subG Γ Σ sub _ _IDENTTGT)
+          (ARROWRA:=@_ARROWRA STT Γ Σ TLRAS)
+          idx init_ths init_ord)
+      ⊢
+      =| 1+idx |=(⟦syn_fairI (1+idx), 1+idx⟧)={E}=>
+        ∃ (γk k γpop γs kt : nat),
+        ⟦syn_tgt_interp_as idx sndl (fun m => s_memory_black m),1+idx⟧ ∗
+        ⟦IsT nTMod idx 1 2 s kt γs,idx⟧ ∗
+        ⟦CInv idx γk k γs γpop,idx ⟧ ∗
+        (* thread_push *)
+        own_thread tid_push ∗
+        ⟦Duty(tid_push) [(k, 0, (dead γk k : sProp idx) ∗ push_then_pop_inv idx γs γpop)],idx⟧ ∗
+        ◇[kt](1, 1) ∗
+        ◇[k](3, 5) ∗
+        live γk (k : nat) (1/2) ∗
+        ⋈[k] ∗
+        (* thread_pop *)
+        GEx γpop tt ∗
+        ◇[kt](1,1) ∗
+        own_thread tid_pop ∗
+        ⟦Duty(tid_pop) [],idx⟧
+  .
+  Proof.
+    iIntros "(Mem & _ & Init)". rewrite red_syn_fairI.
+    iDestruct (memory_init_iprop with "Mem") as "[Mem ↦s]".
+    iDestruct "↦s" as "((s↦ & _) & _)".
+    Local Transparent s.
+    iEval (simpl; fold s) in "s↦".
+    Local Opaque s.
+
+    unfold WSim.initial_prop.
+    iDestruct "Init" as "(_ & _ & Ds & Ts & _ & St_tgt)".
+
+    assert (NatStructsLarge.NatMap.find tid_push init_ths = Some tt) as Htid_push.
+    { unfold init_ths. apply NatStructsLarge.nm_find_add_eq. }
+    iDestruct (natmap_prop_remove_find _ _ _ Htid_push with "Ds") as "[Dpush Ds]".
+    iDestruct (natmap_prop_remove_find _ _ _ Htid_push with "Ts") as "[Tpush Ts]".
+    clear Htid_push.
+
+    assert (NatStructsLarge.NatMap.find tid_pop (NatStructsLarge.NatMap.remove tid_push init_ths) = Some tt) as Htid_pop.
+    { unfold init_ths.
+      rewrite NatStructsLarge.NatMapP.F.remove_neq_o; ss.
+      rewrite NatStructsLarge.nm_find_add_neq; ss.
+      rewrite NatStructsLarge.nm_find_add_eq. ss.
+    }
+    iDestruct (natmap_prop_remove_find _ _ _ Htid_pop with "Ds") as "[Dpop _]".
+    iDestruct (natmap_prop_remove_find _ _ _ Htid_pop with "Ts") as "[Tpop _]".
+    clear Htid_pop.
+
+    iMod (tgt_interp_as_id _ _ (n:=idx) with "[St_tgt Mem]") as "St_tgt"; [auto|..].
+    2:{ iExists _. iFrame. simpl.
+        instantiate (1:=fun '(_, m) => s_memory_black m). simpl.
+        red_tl_all. iFrame.
+    }
+    { simpl. instantiate (1:= (∃ (st : τ{st_tgt_type, idx}), ⟨Atom.ow_st_tgt st⟩ ∗ (let '(_, m) := st in s_memory_black (n:=idx) m))%S).
+      red_tl. f_equal.
+    }
+    iDestruct (tgt_interp_as_compose (n:=idx) (la:=Lens.id) (lb:=sndl) with "St_tgt") as "#TGT_ST".
+    { ss. econs. iIntros ([x m]) "MEM". unfold Lens.view. ss. iFrame.
+      iIntros (m') "MEM". iFrame.
+    }
+    iEval (rewrite Lens.left_unit) in "TGT_ST".
+    iClear "St_tgt". clear.
+
+    iMod (alloc_obligation_fine 3 6) as (k) "(#OB_kb & Pc_k & Po_k)".
+    iEval (rewrite -Qp.half_half) in "Po_k".
+    iDestruct (pending_split _ (1/2) (1/2) with "Po_k") as "(Po_d & Po_p)".
+    iDestruct (pc_split _ _ 5 1 with "Pc_k") as "[Pc_k_push Pc_k]".
+    iMod (pc_drop _ 1 3 ltac:(auto) 1 with "Pc_k") as "Pc_k"; [lia|].
+
+    iMod (Lifetime.alloc k) as (γk) "live".
+    iEval (rewrite -Qp.half_half) in "live".
+    iDestruct (Lifetime.pending_split _ (1/2) (1/2) with "live") as "[live_i live_p]".
+
+    iMod (ghost_excl_alloc tt) as (γpop) "Tok".
+    iMod (alloc_Treiber nTMod idx _ 1 2 with "s↦") as (kt γs) "(#IsT & TStack & Pc_kt)".
+    iDestruct (pc_split _ _ 1 1 with "Pc_kt") as "[? ?]".
+
+    iMod (duty_add _ _ [] _ 0 ((dead γk k : sProp idx) ∗ push_then_pop_inv idx γs γpop : sProp idx)%S with "[$Dpush $Po_d $Pc_k] []") as "Dpush".
+    { simpl. unfold push_then_pop_inv. red_tl_all.
+      rewrite red_syn_inv. iModIntro. iIntros "#$".
+    }
+
+    iDestruct (duty_delayed_tpromise with "Dpush") as "#Prm'"; [ss;eauto|].
+    iMod (activate_tpromise with "Prm' Po_p") as "[#Prm #Act_k]".
+    iClear "Prm'".
+
+    iDestruct (until_tpromise_make1 _ _ _ ((live γk k (1/2) : sProp idx) ∗ TStack idx γs [] : sProp idx)%S with "[live_i TStack]") as "uPrm".
+    { simpl. red_tl_all. iFrame "∗". iFrame "Prm". }
+
+    iMod (FUpd_alloc _ _ _ idx nTCli (CState idx γk k γs γpop) with "[uPrm]") as "#CInv"; [lia| |].
+    { simpl. unfold CState. rewrite red_syn_until_tpromise. iFrame. }
+
+    iModIntro. iExists γk,k,γpop,γs,kt.
+
+    rewrite red_syn_tgt_interp_as. iFrame "∗#".
+    unfold CInv. red_tl. rewrite red_syn_inv. iFrame "OB_kb CInv".
+  Qed.
+
+End INITIAL.
 
 End SPEC.
